LambdaGraph/Subst.lean
@@ -71,19 +71,24 @@ theorem program_subst_size_le {p : Program} {v : Expr} {n : Nat}
     {map : LabelMap p} : p.size ≤ (p.subst map n v).size := by
   simp [Program.subst]
 
-theorem lt_subst_size {p : Program} (v : Expr) {n : Nat} (map : LabelMap p)
-    (hn : n < p.size) : n < (p.subst map n v).size :=
-  Nat.lt_of_lt_of_le hn program_subst_size_le
+theorem lt_subst_size {p : Program} (v : Expr) {m n : Nat} (map : LabelMap p)
+    (hm : m < p.size) : m < (p.subst map n v).size :=
+  Nat.lt_of_lt_of_le hm program_subst_size_le
 
-theorem subst_fn_eq {p : Program} (v : Expr) {m n : Nat} (map : LabelMap p)
-    (hn : m < p.size) :
-    (p.subst map n v).fn[m]'(lt_subst_size v map hn) = p.fn[m] := by
-  simp [hn, Program.subst]
+theorem subst_fn_eq_of_lt {p : Program} (v : Expr) {m n : Nat}
+    (map : LabelMap p) (hm : m < p.size) :
+    (p.subst map n v).fn[m]'(lt_subst_size v map hm) = p.fn[m] := by
+  simp [hm, Program.subst]
+
+theorem subst_fn_eq_of_ge {p : Program} (v : Expr) {m n : Nat}
+    (map : LabelMap p) (hm : p.size ≤ m) (hm' : m < p.size + map.inv.size) :
+    (p.subst map n v).fn[m] = p.fn[map.inv[m - p.size]].subst map n v := by
+  simp [hm, Program.subst]
 
 theorem subst_ty_eq {p : Program} (v : Expr) {m n : Nat} (map : LabelMap p)
-    (hn : m < p.size) :
-    (p.subst map n v).ty[m]'(lt_subst_size v map hn) = p.ty[m] := by
-  simp [hn, Program.subst]
+    (hm : m < p.size) :
+    (p.subst map n v).ty[m]'(lt_subst_size v map hm) = p.ty[m] := by
+  simp [hm, Program.subst]
 
 theorem expr_types_in_subst {p : Program} {e : Expr} (v : Expr) {t : Ty}
     (n : Nat) (map : LabelMap p) (ht : p ⊢ e : t) :
@@ -106,6 +111,7 @@ structure LabelMap.Valid {p : Program} (map : LabelMap p) (n : Nat) : Prop where
   lt : n < p.size
   not_nests : ∀ {i} (h : i < p.size), n ⊁[p] i → map.fwd[i] = i
   nests : ∀ {i} (h : i < p.size), n ≻[p] i → map.ValidNew h
+  fwd_inv : ∀ {k} (h : k < map.inv.size), map.fwd[map.inv[k]] = p.size + k
 
 theorem LabelMap.Valid.eq_or_new {p : Program} {map : LabelMap p} {n : Nat}
     (hmap : map.Valid n) {i : Nat} (hi : i < p.size) :
@@ -124,6 +130,31 @@ theorem LabelMap.Valid.fwd_lt {p : Program} {map : LabelMap p} {n : Nat}
     omega
   · exact h.fwd_lt
 
+theorem LabelMap.Valid.fwd_inj {p : Program} {map : LabelMap p} {n : Nat}
+    (hmap : map.Valid n) {i j : Nat} (hi : i < p.size) (hj : j < p.size)
+    (h : map.fwd[i] = map.fwd[j]) : i = j := by
+  by_cases hni : n ≻[p] i
+  · obtain ⟨hi', hi'', hinvi⟩ := hmap.nests hi hni
+    by_cases hnj : n ≻[p] j
+    · obtain ⟨hj', hj'', hinvj⟩ := hmap.nests hj hnj
+      simp only [h] at hinvi
+      rw [← hinvj, hinvi]
+    · have hj' := hmap.not_nests hj hnj
+      omega
+  · have hi' := hmap.not_nests hi hni
+    by_cases hnj : n ≻[p] j
+    · obtain ⟨hj', hj'', hinvj⟩ := hmap.nests hj hnj
+      omega
+    · have hj' := hmap.not_nests hj hnj
+      rw [← hi', h, hj']
+
+theorem LabelMap.Valid.eq_map_of_ge {p : Program} {map : LabelMap p} {n : Nat}
+    (hmap : map.Valid n) {m : Nat} (hm : p.size ≤ m)
+    (hm' : m < p.size + map.inv.size) : ∃ i : Fin p.size, m = map.fwd[i] := by
+  exists map.inv[m - p.size]
+  rw [hmap.fwd_inv]
+  omega
+
 theorem labelMap_valid (p : Program) {n : Nat} (hn : n < p.size) :
     (p.labelMap n).Valid n where
   lt := hn
@@ -135,6 +166,11 @@ theorem labelMap_valid (p : Program) {n : Nat} (hn : n < p.size) :
     intro i hi h
     unfold Program.labelMap
     exact aux_le_nests hi (Nat.zero_le i) h
+  fwd_inv := by
+    intro i hi
+    unfold Program.labelMap
+    apply aux_fwd_inv
+    simp
 where
   aux_gt_map {i j fwd inv} (hi : i < p.size) (hj : i < j) :
       (Program.labelMap.aux p n j fwd inv).fwd[i] = fwd[i] := by
@@ -165,7 +201,7 @@ where
         omega
       · apply ih
         omega
-  aux_gt_inv {i j k fwd inv} (hk : k < inv.size)
+  aux_gt_inv {j k fwd inv} (hk : k < inv.size)
       (hk' : k < (Program.labelMap.aux p n j fwd inv).inv.size) :
       (Program.labelMap.aux p n j fwd inv).inv[k] = inv[k] := by
     have (eq := hd) d := p.size - j
@@ -217,11 +253,37 @@ where
         have : i = (inv.push ⟨i, hi⟩)[inv.size] := by simp
         conv => rhs; rw [this]
         rw [aux_gt_inv]
-        exact 0 -- what?
     | succ d ih =>
       have hj' : j < p.size := by omega
       simp [hj']
       split <;> apply ih <;> omega
+  aux_fwd_inv {j fwd inv}
+      (h : ∀ k (_ : k < inv.size), ↑inv[k] < j ∧ fwd[inv[k]] = p.size + k) :
+      let ⟨fwd', inv'⟩ := Program.labelMap.aux p n j fwd inv
+      ∀ k (_ : k < inv'.size), fwd'[inv'[k]] = p.size + k := by
+    intro k hk
+    have (eq := hd) d := p.size - j
+    induction d generalizing j fwd inv with unfold Program.labelMap.aux
+    | zero => simp [*, show ¬j < p.size by omega]
+    | succ d ih =>
+      simp only [show j < p.size by omega, ↓reduceDIte, Fin.getElem_fin]
+      split
+      · apply ih
+        · intro k' hk'
+          simp only [Array.size_push] at hk'
+          by_cases k' = inv.size
+          · simp [*]
+          · have : k' < inv.size := by omega
+            obtain ⟨hlt, heq⟩ := h k' this
+            simp only [Fin.getElem_fin] at heq
+            have hne : j ≠ ↑inv[k'] := Ne.symm (Nat.ne_of_lt hlt)
+            simp [*, Array.getElem_push_lt, Nat.lt_succ_of_lt]
+        · omega
+      · apply ih
+        · intro k' hk'
+          obtain ⟨hlt, heq⟩ := h k' hk'
+          simp [*, Nat.lt_succ_of_lt]
+        · omega
 
 theorem subst_ty_map_eq {p : Program} {v : Expr} {m n : Nat} {map : LabelMap p}
     (hm : m < p.size) (hmap : map.Valid n) :
@@ -265,10 +327,43 @@ theorem subst_types {p : Program} {e v : Expr} {t : Ty} {n : Nat}
       exact expr_subst_types (labelMap_valid _ hn) (htp _) htv
   · exact expr_subst_types (labelMap_valid _ hn) ht htv
 
+theorem validRefs_in_subst {p : Program} {e v : Expr} {n : Nat}
+    {map : LabelMap p} (he : e.ValidRefs p) :
+    e.ValidRefs (p.subst map n v) := by
+  induction he with constructor <;> apply_rules [lt_subst_size]
+
+theorem expr_subst_validRefs {p : Program} {e v : Expr} {n : Nat}
+    {map : LabelMap p} (hmap : map.Valid n) (he : e.ValidRefs p)
+    (hv : v.ValidRefs p) : (e.subst map n v).ValidRefs (p.subst map n v) := by
+  induction he with
+    try solve | simp only [Expr.subst]; constructor <;> apply_rules
+  | var m hm =>
+    by_cases h : n = m
+    · simp only [h, Expr.subst, ↓reduceIte]
+      exact validRefs_in_subst hv
+    · simp [*, Expr.subst, ↓reduceIte, getElem?_pos, Option.getD_some]
+      constructor
+      exact hmap.fwd_lt hm
+  | fn =>
+    simp only [*, Expr.subst, getElem?_pos, Option.getD_some]
+    constructor
+    apply hmap.fwd_lt
+
+theorem subst_validRefs {p : Program} {v : Expr} {n : Nat} {map : LabelMap p}
+    (hmap : map.Valid n) (hp : p.ValidRefs) (hv : v.ValidRefs p) :
+    (p.subst map n v).ValidRefs := by
+  intro i hi'
+  by_cases hi : i < p.size
+  · simp [*, subst_fn_eq_of_lt]
+    apply_rules [validRefs_in_subst]
+  · simp only [Nat.not_lt] at hi
+    rw [subst_fn_eq_of_ge _ _ hi]
+    apply expr_subst_validRefs <;> apply_rules
+
 theorem subst_eq_var {p : Program} {e v : Expr} {m n : Nat}
     {map : LabelMap p} (he : e.ValidRefs p) (hc : v.Closed p)
     (h : e.subst map n v = .var m) :
-    ∃ (i : Fin p.size), m = map.fwd[i] ∧ e = .var i := by
+    ∃ i : Fin p.size, m = map.fwd[i] ∧ e = .var i := by
   cases e with simp only [Expr.subst] at h <;> try contradiction
   | var k =>
     have .var _ hk := he
@@ -352,7 +447,7 @@ theorem free_of_free_in_subst {p : Program} {e v : Expr} {m n : Nat}
     constructor
     · exact hne
     · subst p'
-      rw [subst_fn_eq _ _ hk] at ih
+      rw [subst_fn_eq_of_lt _ _ hk] at ih
       exact ih (hp hk)
 
 theorem not_free_in_subst {p : Program} {e v : Expr} {n : Nat}
@@ -369,14 +464,14 @@ theorem not_free_in_subst {p : Program} {e v : Expr} {n : Nat}
     · simp only [Expr.subst, ↓reduceIte] at he'
       subst v
       have .fn _ hm := hv
-      rw [subst_fn_eq _ _ hm] at hf
+      rw [subst_fn_eq_of_lt _ _ hm] at hf
       replace hf := free_of_free_in_subst hp (hp hm) hf
       exact hc n (.fn _ _ hne hf)
     · by_cases hd : n ≻[p] i
       · obtain ⟨hle, hlt, hinv⟩ := hmap.nests hi hd
         exact ih (hp hi) (by simp [*, Program.subst])
       · have hi' := hmap.not_nests hi hd
-        simp only [Fin.getElem_fin, hi', subst_fn_eq _ _ hi] at hf
+        simp only [Fin.getElem_fin, hi', subst_fn_eq_of_lt _ _ hi] at hf
         simp only [Fin.getElem_fin, hi', ne_eq] at hne
         replace hf := free_of_free_in_subst hp (hp hi) hf
         exact hd (.free _ _ hne hf)
@@ -415,7 +510,7 @@ theorem eq_map_of_free_in_subst {p : Program} {e v : Expr} {m n : Nat}
     {map : LabelMap p} (hmap : map.Valid n) (hp : p.ValidRefs)
     (he : e.ValidRefs p) (hv : v.ValidRefs p) (hc : v.Closed p)
     (hvv : v.Value) (hf : (e.subst map n v).Free (p.subst map n v) m) :
-    ∃ (i : Fin p.size), m = map.fwd[i] ∧ e.Free p i := by
+    ∃ i : Fin p.size, m = map.fwd[i] ∧ e.Free p i := by
   generalize hp' : p.subst map n v = p', he' : e.subst map n v = e' at hf
   induction hf generalizing e with
   | var =>
@@ -428,7 +523,7 @@ theorem eq_map_of_free_in_subst {p : Program} {e v : Expr} {m n : Nat}
     · simp only [Expr.subst, ↓reduceIte] at he'
       subst v
       have .fn _ hk := hv
-      rw [subst_fn_eq _ _ hk] at hf
+      rw [subst_fn_eq_of_lt _ _ hk] at hf
       replace hf := free_of_free_in_subst hp (hp hk) hf
       exfalso
       exact hc m (.fn _ _ hne hf)
@@ -440,7 +535,7 @@ theorem eq_map_of_free_in_subst {p : Program} {e v : Expr} {m n : Nat}
           contradiction
         exact ⟨j, rfl, .fn _ hi hij hj⟩
       · obtain hi' := hmap.not_nests hi hd
-        simp only [Fin.getElem_fin, hi', subst_fn_eq v map hi] at hf
+        simp only [Fin.getElem_fin, hi', subst_fn_eq_of_lt v map hi] at hf
         replace hf := free_of_free_in_subst hp (hp hi) hf
         simp [hi'] at hne
         have hm : n ⊁[p] m := fun h => hd (.step _ _ hi hne hf h)
@@ -482,3 +577,97 @@ theorem eq_map_of_free_in_subst {p : Program} {e v : Expr} {m n : Nat}
     have .cond _ _ _ hc het hef := he
     obtain ⟨i, rfl, hf'⟩ := ih hef rfl
     exact ⟨i, rfl, .condF _ _ _ hf'⟩
+
+theorem nests_of_nests_in_subst {p : Program} {m n k : Nat} {v : Expr}
+    {map : LabelMap p} (hk : k < p.size) (hp : p.ValidRefs)
+    (h : m ≻[p.subst map n v] k) : m < p.size ∧ m ≻[p] k := by
+  generalize hp' : p.subst map n v = p' at h
+  induction h with
+  | free k hk' hne hf' =>
+    have hf : p.fn[k].Free p m := by
+      apply free_of_free_in_subst hp (hp hk)
+      subst p'
+      simpa [subst_fn_eq_of_lt _ _ hk] using hf'
+    constructor
+    · exact lt_size_of_free hp (hp hk) hf
+    · apply Nests.free _ hk hne
+      exact hf
+  | step l k hk' hne hf' h ih =>
+    have hf : p.fn[k].Free p l := by
+      apply free_of_free_in_subst hp (hp hk)
+      subst p'
+      simpa [subst_fn_eq_of_lt _ _ hk] using hf'
+    obtain ⟨hm, ih⟩ := ih (lt_size_of_free hp (hp hk) hf)
+    constructor
+    · exact hm
+    · refine Nests.step _ _ hk hne ?_ ih
+      exact hf
+
+theorem nests_of_nests_map_in_subst {p : Program} {m n k : Nat} {v : Expr}
+    {map : LabelMap p} (hk : k < p.size) (hmap : map.Valid n) (hp : p.ValidRefs)
+    (hv : v.ValidRefs p) (hc : v.Closed p) (hvv : v.Value)
+    (h : m ≻[p.subst map n v] map.fwd[k]) :
+    ∃ i : Fin p.size, m = map.fwd[i] ∧ i ≻[p] k := by
+  generalize hp' : p.subst map n v = p', hleq : map.fwd[k] = l at h
+  induction h generalizing k with
+  | free k' hk' hne hf' =>
+    by_cases hnk : n ≻[p] k
+    · subst p' k'
+      obtain ⟨hle, hlt, hinv⟩ := hmap.nests hk hnk
+      simp only [subst_fn_eq_of_ge, Fin.getElem_fin, hle, hinv] at hf'
+      obtain ⟨i, heq, hf⟩ :=
+        eq_map_of_free_in_subst hmap hp (hp _) hv hc hvv hf'
+      refine ⟨i, heq, ?_⟩
+      have : i ≠ k := by
+        intro h
+        subst k
+        contradiction
+      constructor <;> assumption
+    · subst p' k'
+      simp only [hmap.not_nests hk hnk] at *
+      simp only [subst_fn_eq_of_lt, hk] at hf'
+      have hf := free_of_free_in_subst hp (hp hk) hf'
+      have hm := lt_size_of_free hp (hp hk) hf
+      have hnm : n ⊁[p] m := fun h => hnk (Nests.step _ _ _ hne hf h)
+      refine ⟨⟨m, hm⟩, (hmap.not_nests hm hnm).symm, ?_⟩
+      constructor <;> assumption
+  | step l' k' hk' hne hf' h ih =>
+    by_cases hnk : n ≻[p] k
+    · subst p' k'
+      obtain ⟨hle, hlt, hinv⟩ := hmap.nests hk hnk
+      simp only [subst_fn_eq_of_ge, Fin.getElem_fin, hle, hinv] at hf'
+      obtain ⟨l, heq, hf⟩ :=
+        eq_map_of_free_in_subst hmap hp (hp _) hv hc hvv hf'
+      obtain ⟨i, heq', hil⟩ := ih _ heq.symm
+      refine ⟨i, heq', ?_⟩
+      have : l ≠ k := by
+        intro h
+        subst k
+        contradiction
+      apply Nests.step <;> assumption
+    · subst p' k'
+      simp only [hmap.not_nests hk hnk] at *
+      simp only [subst_fn_eq_of_lt, hk] at hf'
+      have hf := free_of_free_in_subst hp (hp hk) hf'
+      have hl := lt_size_of_free hp (hp hk) hf
+      obtain ⟨hm, hml⟩ := nests_of_nests_in_subst hl hp h
+      have hlk : l' ≻[p] k := by constructor <;> assumption
+      have hnl : n ⊁[p] l' := fun h => hnk (nests_trans h hlk)
+      have hnm : n ⊁[p] m := fun h => hnl (nests_trans h hml)
+      exact ⟨⟨m, hm⟩, (hmap.not_nests hm hnm).symm, nests_trans hml hlk⟩
+
+theorem subst_wf  {p : Program} {n : Nat} {v : Expr} {map : LabelMap p}
+    (hmap : map.Valid n) (hp : p.ValidRefs) (hv : v.ValidRefs p)
+    (hc : v.Closed p) (hvv : v.Value) (hwf : p.WF) : (p.subst map n v).WF := by
+  intro m h
+  by_cases hm : m < p.size
+  · obtain ⟨-, h'⟩ := nests_of_nests_in_subst hm hp h
+    exact hwf m h'
+  · simp only [Nat.not_lt] at hm
+    have hp' : (p.subst map n v).ValidRefs := subst_validRefs hmap hp hv
+    have hm' := lt_size_of_nests hp' h
+    obtain ⟨⟨i, hi⟩, rfl⟩ := hmap.eq_map_of_ge hm hm'
+    obtain ⟨⟨j, hj⟩, heq, h'⟩ :=
+      nests_of_nests_map_in_subst hi hmap hp hv hc hvv h
+    simp only [hmap.fwd_inj hi hj heq] at h'
+    exact hwf j h'
